Use a Low* version of blake2_params in Blake2 implementation

code/blake2/Hacl.Impl.Blake2.Core.fsti
@@ -80,6 +80,26 @@ type blake2s_params = {
   personal: lbuffer uint8 8ul;
 }
 
+inline_for_extraction noextract
+let get_blake2s_salt (p: blake2s_params) = p.salt
+
+inline_for_extraction noextract
+let get_blake2s_personal (p: blake2s_params) = p.personal
+
+inline_for_extraction noextract
+let set_blake2s_digest_length
+  (p: blake2s_params)
+  (nn: size_t{1 <= v nn /\ v nn <= Spec.max_output Spec.Blake2S})
+  : blake2s_params =
+  {p with digest_length = to_u8 nn}
+
+inline_for_extraction noextract
+let set_blake2s_key_length
+  (p: blake2s_params)
+  (kk: size_t{v kk <= Spec.max_key Spec.Blake2S})
+  : blake2s_params =
+  {p with key_length = to_u8 kk}
+
 let blake2s_params_inv (h: mem) (p: blake2s_params): GTot prop =
   live h p.salt /\ live h p.personal
 
@@ -143,23 +163,63 @@ let blake2_params (a:Spec.alg) =
   | Spec.Blake2S -> blake2s_params
   | Spec.Blake2B -> blake2b_params
 
+inline_for_extraction noextract
+let set_digest_length (#a: Spec.alg)
+  (p: blake2_params a)
+  (nn: size_t{1 <= v nn /\ v nn <= Spec.max_output a})
+  : blake2_params a =
+  match a with
+  | Spec.Blake2S -> set_blake2s_digest_length p nn
+  | Spec.Blake2B -> {p with digest_length = to_u8 nn}
+
+inline_for_extraction noextract
+let set_key_length (#a: Spec.alg)
+  (p: blake2_params a)
+  (kk: size_t{v kk <= Spec.max_key a})
+  : blake2_params a =
+  match a with
+  | Spec.Blake2S -> set_blake2s_key_length p kk
+  | Spec.Blake2B -> {p with key_length = to_u8 kk}
+
+inline_for_extraction noextract
+let get_salt (#a: Spec.alg) (p: blake2_params a) : lbuffer uint8 (salt_len a) =
+  match a with
+  | Spec.Blake2S -> get_blake2s_salt p
+  | Spec.Blake2B -> p.salt
+
+inline_for_extraction noextract
+let get_personal (#a: Spec.alg) (p: blake2_params a) : lbuffer uint8 (personal_len a) =
+  match a with
+  | Spec.Blake2S -> get_blake2s_personal p
+  | Spec.Blake2B -> p.personal
+
 noextract inline_for_extraction
-let blake2_params_inv (a:Spec.alg) (h: mem) (p: blake2_params a) =
+let blake2_params_inv (#a:Spec.alg) (h: mem) (p: blake2_params a) =
   match a with
   | Spec.Blake2S -> blake2s_params_inv h p
   | Spec.Blake2B -> blake2b_params_inv h p
 
 noextract inline_for_extraction
-let blake2_params_loc (a:Spec.alg) (p: blake2_params a) =
+let blake2_params_loc (#a:Spec.alg) (p: blake2_params a) =
   match a with
   | Spec.Blake2S -> blake2s_params_loc p
   | Spec.Blake2B -> blake2b_params_loc p
 
 noextract inline_for_extraction
-let blake2_params_v (a:Spec.alg) (h: mem) (p: blake2_params a) : GTot (Spec.blake2_params a) =
+let blake2_params_v (#a:Spec.alg) (h: mem) (p: blake2_params a) : GTot (Spec.blake2_params a) =
   match a with
   | Spec.Blake2S -> blake2s_params_v h p
   | Spec.Blake2B -> blake2b_params_v h p
+
+noextract inline_for_extraction
+val alloc_default_params: a:Spec.alg ->
+	  StackInline (blake2_params a)
+	  (requires (fun h -> True))
+	  (ensures (fun h0 p h1 ->
+            stack_allocated (get_salt p) h0 h1 (Lib.Sequence.create (Spec.salt_length a) (u8 0)) /\
+            stack_allocated (get_personal p) h0 h1 (Lib.Sequence.create (Spec.personal_length a) (u8 0)) /\
+            blake2_params_inv h1 p /\
+            blake2_params_v h1 p == Spec.blake2_default_params a))
 
 noextract inline_for_extraction
 unfold let state_p (a:Spec.alg) (m:m_spec) =
